---
date: 2022-01-13
title: "The C method"
subtitle: "An analytical knee/elbow searching method"
tags:
  - math
  - machine-learning
  - optimization
grammarly_score_start: 67
grammarly_score_end: 84
---
Knee searching is quite important operation. Here I describe the method I personally developed: the so-called **C-method**.

## Description

It all started with an observation: many tradeoff curves I've come across with vaguely look like $`\frac1x`$ or $`1-\frac1x`$. The most generic form of this equation is:

```math
f\left(x\right) = a+ \frac{b}{x+c}
```

It has three shape parameters: $`a`$, $`b`$, and $`c`$, and fitting these parameters should be enough. However, I felt that this is way too much degrees of freedom; if I restrict the function with some constraints, I should ideally get the functional form with only one shape parameter. The restrictions I came up with is to anchor the function such that $`f(0) = 0`$ and $`f(1) = 1`$.

### Constraint 1
When $`f(0)=0`$ is fed into the equation form results in a relation:
```math
\begin{align*}
0 = f(0) &= a+\frac{b}{0+c} =\\
         &= a+\frac{b}c =\\
         &\Leftrightarrow =\\
       b &= -ac \\
\end{align*}
```
which is cute and simple. Feeding the relation back into the equation results with:
```math
\begin{align*}
    f(x) &= a - \frac{ac}{x+c} =\\
         &= a\left(1 - \frac{c}{x+c}\right) =\\
         &= a\left(\frac{x+c}{x+c} - \frac{c}{x+c}\right) =\\
         &= \frac{ax}{x+c}
\end{align*}
```
Nice and simple

### Constaint 2
Feeding $`f(1)=1`$ gets us a quick win:
```math
\begin{align*}
1 = f(1) &= \frac{a}{1+c} \Leftrightarrow \\
       a &= 1+c \\
\end{align*}
```
and feeding it back results in:
```math
f(x) = \frac{\left(1+c\right)x}{x+c}
```

## Analysis
The result has several properties:
1. $`\lim_{c \rightarrow 0} = 1`$
2. $`\lim_{c \rightarrow +\infty} = x`$
3. When $`c \lt 0`$, the curve "flips", meaning the curve avoids the unit square.

I decided I did not like this as, while perfectly mathematically correct, it's not match my intuition at all :sweat_smile: to me, ideally $`\lim_{c \rightarrow 0}`$ should go to $`x`$ and $`\lim_{c \rightarrow +\infty}`$ should go to $`x`$. Also, I would like to restrict $`c`$ to all positive reals.

## Better solution
All of my problems are solved with a following substitution: $`c \rightarrow \frac1{e^c}`$. Mathematicians probably hate me right now. Anyhow, doing the substitution gave me:
```math
\begin{align*}
f(x) = \frac{\left(1+c\right)x}{x+c} &\rightarrow \frac{\left(1+\frac1{e^c}\right)x}{x+\frac1{e^c}} = \\
    &= \frac{x\left(e^c+1\right)}{xe^c + 1}\\
\end{align*}
```
Much better, IMHO. It's got a nice visual which is easy to remember. The only difference is the parantheses :smile:

The animation of the function image

### Analysis
1. $`\lim_{c \rightarrow -\infty} = x`$, which was what I wanted
2. $`\lim_{c \rightarrow +\infty} = 1`$, which was also what I wanted
3. Flipping is now disabled

## How to use it to find a knee?
Three ways: the intuitive way, the technical way, and the hacky way.

### The intuitive way
The intuitive way starts with an observation that the function graph is symmetric with respect to the line $`y=1-x`$. Intersecting the graph with the line gives:
```math
\begin{align*}
1-x &= \frac{x\left(e^c+1\right)}{xe^c+1} \\
\left(1-x\right)\left(xe^c+1\right) &= x\left(e^c+1\right) \\
e^cx+1-e^cx^2-e^cx-x&=0 \\
e^cx^2+2x-1&=0 \\
\end{align*}
```

The quadratic equation has two solutions, however I must disregard one of them as it's smaller than $`0`$. Therefore, the knee point is at:
```math
x=\frac{-1+\sqrt{1+e^c}}{e^c}
```

### The technical way
The second way is way more technical as it involves a lot of calculus. If I define a curvature function $`K(x)=\frac{f''}{\left(1+f'^2\right)^\frac32}`$, I could find an extreme point by $`\frac{d}{dx}K\left(x\right) = 0`$. Before substitution, let's play with the expression first:
```math
\begin{align*}
\frac{d}{dx}K\left(x\right) &= \frac{d}{dx}\left(\frac{f''}{\left(1+f'^2\right)^\frac32}\right) = 0 \\
\frac{d}{dx}f''\cdot\left(1+f'^2\right)^{\frac32} &= f''\cdot\frac{d}{dx}\left(\left(1+f'^2\right)^{\frac32}\right) \\
f'''\left(1+f'^2\right)^{\frac32} &= f''\cdot\frac32\left(1+f'^2\right)^{\frac12}\cdot2f'f''\\
f'''\left(1+f'^2\right) &= 3f''^2f' \\
\end{align*}
```

The higher derivatives of $`f(x)`$ are as follows:
```math
\begin{align*}
f(x) &= \frac{x\left(e^c+1\right)}{xe^c+1} \\
f'(x) = \frac{d}{dx}f(x)&=\frac{e^c+1}{\left(xe^c+1\right)^2} \\
f''(x) = \frac{d}{dx}f'(x)&=-\frac{2e^c\left(e^c+1\right)}{\left(xe^c+1\right)^3} \\
f'''(x) = \frac{d}{dx}f''(x)&=\frac{6e^{2c}\left(e^c+1\right)}{\left(xe^c+1\right)^4} \\
\end{align*}
```
Substituting these equations leads to:
```math
\begin{align*}
f'''\left(1+f'^2\right) &= 3f''^2f' & \textit{substitute the derivatives}\\
\frac{6e^{2c}\left(e^c+1\right)}{\left(xe^c+1\right)^4}\left(1+\left(\frac{e^c+1}{\left(xe^c+1\right)^2}\right)^2\right) &= 3\left(-\frac{2e^c\left(e^c+1\right)}{\left(xe^c+1\right)^3}\right)^2\frac{e^c+1}{\left(xe^c+1\right)^2} & \textit{expand}\\
\frac{6e^{2c}\left(e^c+1\right)}{\left(xe^c+1\right)^4}\frac{\left(xe^c+1\right)^4 + \left(e^c+1\right)^2}{\left(xe^c+1\right)^4} &= 12\frac{e^{2c}\left(e^c+1\right)^2}{\left(xe^c+1\right)^6}\frac{e^c+1}{\left(xe^c+1\right)^2} & \textit{a lot of things cancel out}\\
\left(xe^c+1\right)^4+\left(e^c+1\right)^2 &= 2\left(e^c+1\right)^2 \\
\left(xe^c+1\right)^4 &= 2\left(e^c+1\right)^2 & \textit{take the positive square root} \\
\left(xe^c+1\right)^2 &= e^c+1 \\
xe^c+1 &= \sqrt(e^c+1) \\
x &= \frac{\sqrt{e^c+1}-1}{e^c} \\
\end{align*}
```
which is what we've already obtained in the last step, which is great!

### The hacky way
The third approach is rather hacky. By invoking a [Mean Value Theorem](https://en.wikipedia.org/wiki/Mean_value_theorem), we know there must be a point on the curve of $`f(x)`$ in which the slope of the tangent is equal to the slope of the secant between $`(0, 0`$ and $`(1, 1)`$. That slope is, obviously, 1. Therefore, finding the derivative and evaluating it with 1 gives:
```math
\begin{align*}
\frac{d}{dx}f(x) &= 1 \\
\frac{d}{dx}\frac{x\left(e^c+1\right)}{xe^c+1} &= 1 \\
\frac{e^c+1}{\left(xe^c+1\right)^2} &= 1\\
\end{align*}
```
which, once again, results with $`x = \frac{\sqrt{e^c+1}-1}{e^c}`$.

After three different proofs, I guess it's safe to say that $`x = \frac{\sqrt{e^c+1}-1}{e^c}`$ is a good estimator of the theoretical knee.

## Estimating the c
After this theoretical derivation, the next problem is fitting the $`c`$ coefficient to the real world data, $`N`$-dimensional vectors $`\textbf{x}`$ and $`\textbf{y}`$. The first, and only insofar, fitting procedure I've come up with is the ordinary least squares: minimization of:

```math
E = \sum_{i=1}^{N}{\left(y_i - f(x_i)\right)^2} = \sum_{i=1}^{N}{\left(y_i - \frac{x_i\left(e^c+1)\right)}{x_ie^c+1}\right)^2} 
```

I've implemented a $`c`$-fitting procedure in my project called [knarrow](https://github.com/InCogNiTo124/knarrow.git) in the form of the Newton-Raphson method.
```math
\begin{align*}
\frac{\partial E}{\partial c} &= \frac{\partial}{\partial c}\left(\sum_{i=1}^N{\left(y_i - f(x_i)\right)^2}\right) \\
&= 2 \sum_{i=1}^N{\left(f(x_i)-y_i\right)\frac{\partial}{\partial c}f(x_i)}\\
&= 2 \sum_{i=1}^N{\left(y_i-\frac{x_i\left(e^c+1\right)}{x_ie^c+1}\right)}\frac{\left(x_i-1\right)x_i\mathrm{e}^c}{\left(x_i\mathrm{e}^c+1\right)^2}\\

\frac{\partial^2 E}{\partial c^2} &= \frac{\partial^2}{\partial c^2}\left(\sum_{i=1}^N{\left(y_i - f(x_i)\right)^2}\right) \\
&= 2\sum_{i=1}^N{\left(\frac{\partial}{\partial c}f(x_i)\right)^2} + 2\sum_{i=1}^N{\left(f(x_i) - y_i\right)\frac{\partial^2}{\partial c^2}f(x_i)} \\
&= 2\sum_{i=1}^N{\left(\frac{x_i\left(e^c+1\right)}{x_ie^c+1}\right)^2 + \left(\frac{x_i\left(e^c+1\right)}{xe^c+1}-y_i\right)\dfrac{\left(x_i-1\right)x_i\mathrm{e}^c\left(x_i\mathrm{e}^c-1\right)}{\left(x_i\mathrm{e}^c+1\right)^3}}\\
\end{align*}
```

These equations are then simply converted to an update rule:
```math
c_{n+1} \leftarrow c_n - \frac{\frac{\partial E}{\partial c}}{\frac{\partial^2 E}{\partial c^2}}
```
which works for any starting value $`c_0`$. This procedure is repeated until a satisfactory level of precision is reached. The resulting shape parameter $`c`$ is then fed into the equation above to get the knee point. Optionally, one can also calculate which of the input x's is the closest to the theoretical knee and denote that particular x as a kne.

## What's next?
- I would be most happy if I found that $`f'(x)`$ could be written in terms of $`f(x)`$ or $`f''(x)`$ could be written in terms of $`f'(x)`$ in a nice manner (just like the derivative of a sigmoid). However, I am not _that_ good in algebra.
- Efficient implementation. Currenctly it's implemented as a brain-dead _verbatim_ implementation using only numpy. I'm even calling other functions to calculate the derivatives, which turned out to be rather slow. If I ever accomplished the point above, this would easily follow.
- Sometimes, the graphs which are in need of the knee/elbow search do not behave like $`1-\frac1x`$ but more like $`1-\frac1{x^2}`$ or $`1-\frac1{\sqrt{x}}`$. It would be great to investigate such possibilities and allow for one more shape parameter.
